\documentclass[11pt, reqno]{article}

\usepackage{amsmath, amsthm, amssymb}
\usepackage{enumitem}
\usepackage{bookmark}
\usepackage{fullpage}
\usepackage{tcolorbox}
\usepackage{hyperref}
\usepackage{tikz}
\usetikzlibrary{arrows.meta}
\usepackage{pdfpages}
\usepackage{mathrsfs}
\usepackage{fancyhdr}
\usepackage[bottom=0.5in, top=1in, left=0.5in, right=0.5in]{geometry}
\usepackage{array}   % for \newcolumntype macro
\newcolumntype{L}{>{$}l<{$}}

\begin{document}


\topmargin=-40pt
\rhead{Henry Woodburn}
\lhead{Math 653}
\renewcommand{\headrulewidth}{1pt}
\renewcommand{\headsep}{20pt}
\thispagestyle{fancy}

\section*{Homework 1}

\begin{enumerate}
    \item Let $G$ be a group, $H \subset G$ be a subgroup, and $g \in G$. We will show
    $gHg^{-1} = \{ghg^{-1}: h \in H\}$ is a subgroup. 

    It contains the identity since $geg^{-1} = gg^{-1} = e$. 
    
    It contains inverses: let $gag^{-1}$
    be some element of $gHg^{-1}$, with $a \in H$. Then since $H$ is a subgroup, $a^{-1} \in H$, 
    and $ga^{-1}g^{-1} \in gHg^{-1}$ is the inverse of $gag^{-1}$ since $gag^{-1}ga^{-1}g^{-1}
    = gaa^{-1}g^{-1} = e$.

    Finally, $gHg^{-1}$ is closed under multiplication since for $gag^{-1}, gbg^{-1} \in gHg^{-1}$,
    $gag^{-1}gbg^{-1} = gabg^{-1}$. As $H$ is a subgroup, we have $ab \in H$ and thus $gabg^{-1} \in gHg^{-1}$.

    Now we show that $gHg^{-1}$ is isomorphic to $H$. I claim the map $\varphi: H \rightarrow gHg^{-1}$
    defined by $a \mapsto gag^{-1}$ is an isomorphism of subgroups. It is a group homomorphism
    since $\varphi(ab) = gabg^{-1} = gag^{-1}gbg^{-1} = \varphi(a)\varphi(b)$. It is injective: 
    suppose $\varphi(a) = e$. Then $gag^{-1} = e$, and thus $a = g^{-1}eg = e$. It is surjective: 
    choose any $gag^{-1} \in gHg^{-1}$. Then $\varphi(a) = gag^{-1}$. Thus $\varphi$ is an isomorphism.
    
\end{enumerate}

\end{document}